Fix ZXCALC instance and example VyZX diagram

theories/GraphCore/TensorGraphExamples.v
@@ -1,18 +1,17 @@
-Require Export TensorGraphSemantics.
-
+Require Export TensorGraphSemantics ZXGraph.
+Local Open Scope positive_scope.
 
 (* Definition example_graph : TensorGraph (R:=C) (A:=bool) :=
   ∅G +[ 1 := (fun n m => @zsp n m 0) ]
      +[ 3 := (fun n m => @zsp n m 0) ]
-     +{ (1,2) ; (1,3) ; (1,2) ; (1,3) ; (1,4) }.
+     +{ (1,2) ; (1,3) ; (1,2) ; (1,3) ; (1,4) }. *)
 
 
-Definition example_graph' : TensorGraph (R:=C) (A:=bool) :=
-  ∅G +[ 1 := (fun n m => @zsp n m 0) ]
-     +[ 3 := (fun n m => @zsp n m 0) ]
-     +{ (1,2) ; (1,3) ; (3,4) }.
+Definition example_graph' : CospanHyperGraph (bool*R) 0 2 :=
+  [#] -> {[ 1 := ((false, 0%R), [], [2;1]) ; 
+        3 := ((false, 0%R), [1], [3])]} <- [# 2;3].
 
-Compute graph_tensorlist_semantics example_graph.
+(* Compute graph_tensorlist_semantics example_graph.
 
 Compute elements $ inputs example_graph.
 
@@ -25,61 +24,27 @@ Compute elements $ inputs example_graph'.
 Compute elements $ outputs example_graph'. *)
 
 
-(*
+Import ZXCore.
 From VyZX Require Import CoreData.
 
 Open Scope ZX_scope.
 
 Open Scope nat_scope.
 
-Example example_graph'_map_semantics : forall b b',
-  graph_map_semantics example_graph'
-    ∅ {[2:=b; 4:=b']} =
+Example example_graph'_semantics : forall b b',
+  graph_semantics example_graph'
+    [#] [#b;b'] =
   ⟦ Z 0 2 0 ⟷ (— ↕ Z 1 1 0) ⟧
     (Bits.funbool_to_nat 2 ([b;b'] !!!.)) O.
 Proof.
-  cbn -[graph_map_semantics].
+  cbn -[graph_semantics].
   unfold kron.
-  cbn -[graph_map_semantics].
-  intros [] []; cbn -[graph_map_semantics]; (etransitivity;
-    [unfold example_graph';
-      remember @zsp as zsp' eqn:Hzsp;
-      vm_compute|Csimpl; reflexivity]);
-  subst zsp'; cbn -[Cexp];
-  change R0 with 0%R; rewrite ?Cexp_0; lca.
-Qed.
+  cbn -[graph_semantics].
+  intros [] []; cbn -[graph_semantics]; (etransitivity;
+    [unfold example_graph', ZXCALC;
 
-Example example_graph'_list_semantics : forall b b',
-  graph_list_semantics example_graph'
-    [] [b; b'] =
-  ⟦ Z 0 2 0 ⟷ (— ↕ Z 1 1 0) ⟧
-    (Bits.funbool_to_nat 2 ([b;b'] !!!.)) O.
-Proof.
-  cbn -[graph_list_semantics].
-  unfold kron.
-  cbn -[graph_list_semantics].
-  intros [] []; cbn -[graph_list_semantics]; (etransitivity;
-    [unfold example_graph';
       remember @zsp as zsp' eqn:Hzsp;
       vm_compute|Csimpl; reflexivity]);
   subst zsp'; cbn -[Cexp];
   change R0 with 0%R; rewrite ?Cexp_0; lca.
 Qed.
-
-Example example_graph'_vector_semantics : forall b b',
-  graph_vector_semantics example_graph'
-    [# ] [# b; b'] =
-  ⟦ Z 0 2 0 ⟷ (— ↕ Z 1 1 0) ⟧
-    (Bits.funbool_to_nat 2 ([b;b'] !!!.)) O.
-Proof.
-  cbn -[graph_vector_semantics].
-  unfold kron.
-  cbn -[graph_vector_semantics].
-  intros [] []; cbn -[graph_vector_semantics]; (etransitivity;
-    [unfold example_graph';
-      remember @zsp as zsp' eqn:Hzsp;
-      vm_compute|Csimpl; reflexivity]);
-  subst zsp'; cbn -[Cexp];
-  change R0 with 0%R; rewrite ?Cexp_0; lca.
-Qed.
- *)
